feat(KSA): DoNotVersion for Initialize Mutation (#1082)

AwsCryptographicMaterialProviders/dafny/AwsCryptographyKeyStoreAdmin/src/InitializeMutation.dfy
@@ -64,20 +64,13 @@ module {:options "/functionSyntax:4" } InternalInitializeMutation {
       output.Success?
       ==>
         && StateStrucs.ValidMutations?(input.Mutations)
+        && 0 < |input.Identifier|
     ensures
       && output.Success?
       && input.Mutations.TerminalKmsArn.Some?
       ==>
         && KmsArn.ValidKmsArn?(input.Mutations.TerminalKmsArn.value)
-    ensures
-      && output.Success?
-      ==>
-        input.DoNotVersion == false
   {
-    :- Need(
-         input.DoNotVersion == false,
-         Types.UnsupportedFeatureException(message := "At this time, DoNotVersion MUST be false.")
-       );
     :- Need(|input.Identifier| > 0,
             Types.KeyStoreAdminException(message := "Branch Key Identifier cannot be empty!"));
     var terminalEC := input.Mutations.TerminalEncryptionContext.UnwrapOr(map[]);
@@ -298,7 +291,7 @@ module {:options "/functionSyntax:4" } InternalInitializeMutation {
     assert MutationToApply.Original.customEncryptionContext.Keys !! Structure.BRANCH_KEY_RESTRICTED_FIELD_NAMES;
     assert MutationToApply.Terminal.customEncryptionContext.Keys !! Structure.BRANCH_KEY_RESTRICTED_FIELD_NAMES;
     assert MutationToApply.ValidState();
-    // -= BEGIN Version Active Branch Key
+
     // --= Validate Active Branch Key
     var verifyActive? := Mutations.VerifyEncryptedHierarchicalKey(
       item := activeItem,
@@ -330,68 +323,17 @@ module {:options "/functionSyntax:4" } InternalInitializeMutation {
           + " For Initialize Mutation to succeed, the ACTIVE & Beacon Key MUST be in the original state."
       ));
 
-    // --= Generate New Decrypt Only Branch Key with terminal properties
-    var maybeNewVersion := UUID.GenerateUUID();
-    var newVersion :- maybeNewVersion
-    .MapFailure(e => Types.KeyStoreAdminException(
-                    message := "Could not generate UUID for new Decrypt Only. " + e));
 
+    var initializeMutationActiveInput := InitializeMutationActiveInput(
+      input := input,
+      activeItem := activeItem,
+      mutationToApply := MutationToApply,
+      timestamp := timestamp);
+    assert initializeMutationActiveInput.ValidState();
+    var initializeMutationActiveOutput :- InitializeMutationActive(initializeMutationActiveInput);
 
-    var decryptOnlyEncryptionContext := Mutations.DecryptOnlyBranchKeyEncryptionContextForMutation(
-      input.Identifier,
-      newVersion,
-      timestamp,
-      input.logicalKeyStoreName,
-      MutationToApply.Terminal.kmsArn,
-      MutationToApply.Terminal.customEncryptionContext
-    );
-
-    // TODO-Mutations-GA? :: If the KMS Call fails with access denied,
-    // it indicates that the MPL Consumer does not have access to
-    // GenerateDataKeyWithoutPlaintext on the terminal key.
-    var newDecryptOnly :- CreateNewTerminalDecryptOnlyBranchKey(
-      decryptOnlyEncryptionContext,
-      MutationToApply,
-      input.keyManagerStrategy
-    );
-
-    var ActiveEncryptionContext := Structure.ActiveBranchKeyEncryptionContext(newDecryptOnly.EncryptionContext);
-
-    var newActive;
-    if (input.keyManagerStrategy.decryptEncrypt?) {
-      newActive :- Mutations.NewActiveItemForDecryptEncrypt(
-        item := newDecryptOnly,
-        terminalKmsArn := MutationToApply.Terminal.kmsArn,
-        terminalEncryptionContext := ActiveEncryptionContext,
-        keyManagerStrategy := input.keyManagerStrategy,
-        localOperation := "InitializeMutation"
-      );
-    } else {
-      newActive :- Mutations.ReEncryptHierarchicalKey(
-        item := newDecryptOnly,
-        originalKmsArn := MutationToApply.Terminal.kmsArn,
-        terminalKmsArn := MutationToApply.Terminal.kmsArn,
-        terminalEncryptionContext := ActiveEncryptionContext,
-        keyManagerStrategy := input.keyManagerStrategy,
-        localOperation := "InitializeMutation");
-    }
     // -= Mutate Beacon Key
-    var BeaconEncryptionContext := Structure.ReplaceMutableContext(
-      readItems.BeaconItem.EncryptionContext,
-      MutationToApply.Terminal.kmsArn,
-      MutationToApply.Terminal.customEncryptionContext
-    );
-
-    assert readItems.BeaconItem.KmsArn == MutationToApply.Original.kmsArn;
-
-    var newBeaconKey :- Mutations.ReEncryptHierarchicalKey(
-      item := readItems.BeaconItem,
-      originalKmsArn := MutationToApply.Original.kmsArn,
-      terminalKmsArn := MutationToApply.Terminal.kmsArn,
-      terminalEncryptionContext := BeaconEncryptionContext,
-      keyManagerStrategy := input.keyManagerStrategy,
-      localOperation := "InitializeMutation"
-    );
+    var newBeaconKey :- Mutations.MutateItem(readItems.BeaconItem, MutationToApply, input.keyManagerStrategy, "InitializeMutation", false);
 
     // -= Create Mutation Commitment & Mutation Index
     var MutationCommitment :- StateStrucs.SerializeMutationCommitment(MutationToApply);
@@ -404,17 +346,23 @@ module {:options "/functionSyntax:4" } InternalInitializeMutation {
     // -= Write Mutation Commitment, new branch key version, mutated beacon key
     var throwAway2? := input.storage.WriteInitializeMutation(
       KeyStoreTypes.WriteInitializeMutationInput(
-        Active := KeyStoreTypes.OverWriteEncryptedHierarchicalKey(Item:=newActive, Old:=activeItem),
-        Version := KeyStoreTypes.WriteInitializeMutationVersion.rotate(rotate:=newDecryptOnly),
+        Active := initializeMutationActiveOutput.writeActive,
+        Version := initializeMutationActiveOutput.writeVersion,
         Beacon := KeyStoreTypes.OverWriteEncryptedHierarchicalKey(Item:=newBeaconKey, Old:=readItems.BeaconItem),
-        MutationCommitment :=  SignedMutationCommitment, // MutationCommitment,
-        MutationIndex := SignedMutationIndex // MutationIndex
+        MutationCommitment :=  SignedMutationCommitment,
+        MutationIndex := SignedMutationIndex
       ));
     // TODO-Mutations-FF :: Ideally, we would diagnosis the Storage Failure.
     // What Condition Check failed? Was the Key Versioned? Or did another M-Commitment get written?
     var _ :- throwAway2?.MapFailure(e => Types.Error.AwsCryptographyKeyStore(e));
 
-    var mutatedBranchKeyItems := GetMutatedBranchKeyItems(mutationCommitmentUUID, newVersion);
+    var logStatements :=
+      [
+        Types.MutatedBranchKeyItem(ItemType := "Mutation Commitment: " + mutationCommitmentUUID, Description := "Created"),
+        Types.MutatedBranchKeyItem(ItemType := "Mutation Index: " + mutationCommitmentUUID, Description := "Created")
+      ]
+      + initializeMutationActiveOutput.logStatements
+      + [Types.MutatedBranchKeyItem(ItemType := "Beacon", Description := "Mutated")];
 
     var Token := Types.MutationToken(
       Identifier := input.Identifier,
@@ -425,19 +373,8 @@ module {:options "/functionSyntax:4" } InternalInitializeMutation {
 
     return Success(Types.InitializeMutationOutput(
                      MutationToken := Token,
-                     MutatedBranchKeyItems := mutatedBranchKeyItems,
+                     MutatedBranchKeyItems := logStatements,
                      InitializeMutationFlag := Flag));
-  }
-
-  function GetMutatedBranchKeyItems(mutationCommitmentUUID: seq<char>, newVersion: seq<char>)
-    : (output: seq<Types.MutatedBranchKeyItem>)
-  {
-    [Types.MutatedBranchKeyItem(ItemType := "Mutation Commitment: " + mutationCommitmentUUID, Description := "Created"),
-     Types.MutatedBranchKeyItem(ItemType := "Mutation Index: " + mutationCommitmentUUID, Description := "Created"),
-     Types.MutatedBranchKeyItem(ItemType := "Active: " + newVersion, Description := "Created"),
-     Types.MutatedBranchKeyItem(ItemType := "Decrypt Only: " + newVersion, Description := "Created"),
-     Types.MutatedBranchKeyItem(ItemType := "Beacon", Description := "Mutated")
-    ]
   }
 
   method {:isolate_assertions} CreateNewTerminalDecryptOnlyBranchKey(
@@ -609,5 +546,221 @@ module {:options "/functionSyntax:4" } InternalInitializeMutation {
                      MutatedBranchKeyItems := mutatedBranchKeyItems,
                      InitializeMutationFlag := Flag));
 
+  }
+
+  datatype InitializeMutationActiveInput =
+    | InitializeMutationActiveInput (
+        nameonly input: InternalInitializeMutationInput,
+        nameonly activeItem: KeyStoreTypes.EncryptedHierarchicalKey,
+        nameonly mutationToApply: StateStrucs.MutationToApply,
+        nameonly timestamp: string
+      )
+  {
+    ghost predicate ValidState()
+    {
+      && input.ValidState()
+      && activeItem.Type.ActiveHierarchicalSymmetricVersion?
+      && mutationToApply.ValidState()
+      && 0 < |timestamp|
+      && 0 < |input.Identifier|
+      && activeItem.KmsArn == mutationToApply.Original.kmsArn
+      && Structure.EncryptedHierarchicalKey?(activeItem)
+    }
+
+    ghost const Modifies :=
+      match input.keyManagerStrategy {
+        case reEncrypt(km) => multiset(km.kmsClient.Modifies)
+        case decryptEncrypt(kmD, kmE) => multiset(kmD.kmsClient.Modifies) + multiset(kmE.kmsClient.Modifies)
+      }
+      + multiset(input.SystemKey.Modifies)
+      + multiset(input.storage.Modifies)
+  }
+
+  datatype InitializeMutationActiveOutput =
+    | InitializeMutationActiveOutput(
+        nameonly writeActive: KeyStoreTypes.OverWriteEncryptedHierarchicalKey,
+        nameonly writeVersion: KeyStoreTypes.WriteInitializeMutationVersion,
+        nameonly logStatements: seq<Types.MutatedBranchKeyItem>
+      )
+  {
+    ghost predicate ValidState()
+    {
+      && |logStatements| == 2
+    }
+  }
+
+  method InitializeMutationActive(
+    localInput: InitializeMutationActiveInput
+  )
+    returns (output: Result<InitializeMutationActiveOutput, Types.Error>)
+    requires localInput.ValidState()
+    modifies localInput.Modifies
+    ensures localInput.ValidState()
+    ensures
+      && localInput.input.DoNotVersion
+      && output.Success?
+      ==>
+        output.value.writeVersion.mutate?
+    ensures
+      && !localInput.input.DoNotVersion
+      && output.Success?
+      ==>
+        output.value.writeVersion.rotate?
+    ensures output.Success? ==> output.value.ValidState()
+  {
+    if (localInput.input.DoNotVersion) {
+      output := InitializeMutationActiveMutate(localInput);
+    } else {
+      output := InitializeMutationActiveVersion(localInput);
+    }
+    return output;
+  }
+
+  method InitializeMutationActiveVersion(
+    localInput: InitializeMutationActiveInput
+  )
+    returns (output: Result<InitializeMutationActiveOutput, Types.Error>)
+    requires localInput.ValidState()
+    modifies localInput.Modifies
+    ensures localInput.ValidState()
+    requires !localInput.input.DoNotVersion
+    ensures
+      output.Success?
+      ==>
+        && output.value.ValidState()
+        && output.value.writeVersion.rotate?
+        && output.value.logStatements[0].Description == "Rotated"
+        && |output.value.logStatements| == 2
+  {
+    // --= Generate New Decrypt Only Branch Key with terminal properties
+    var maybeNewVersion := UUID.GenerateUUID();
+    var newVersion :- maybeNewVersion
+    .MapFailure(e => Types.KeyStoreAdminException(
+                    message := "Could not generate UUID for new Decrypt Only. " + e));
+
+
+    var decryptOnlyEncryptionContext := Mutations.DecryptOnlyBranchKeyEncryptionContextForMutation(
+      localInput.input.Identifier,
+      newVersion,
+      localInput.timestamp,
+      localInput.input.logicalKeyStoreName,
+      localInput.mutationToApply.Terminal.kmsArn,
+      localInput.mutationToApply.Terminal.customEncryptionContext
+    );
+
+    // TODO-Mutations-GA? :: If the KMS Call fails with access denied,
+    // it indicates that the MPL Consumer does not have access to
+    // GenerateDataKeyWithoutPlaintext on the terminal key.
+    var newDecryptOnly :- CreateNewTerminalDecryptOnlyBranchKey(
+      decryptOnlyEncryptionContext,
+      localInput.mutationToApply,
+      localInput.input.keyManagerStrategy
+    );
+
+    var ActiveEncryptionContext := Structure.ActiveBranchKeyEncryptionContext(newDecryptOnly.EncryptionContext);
+
+    var newActive;
+    if (localInput.input.keyManagerStrategy.decryptEncrypt?) {
+      newActive :- Mutations.NewActiveItemForDecryptEncrypt(
+        item := newDecryptOnly,
+        terminalKmsArn := localInput.mutationToApply.Terminal.kmsArn,
+        terminalEncryptionContext := ActiveEncryptionContext,
+        keyManagerStrategy := localInput.input.keyManagerStrategy,
+        localOperation := "InitializeMutation"
+      );
+    } else {
+      var input := Mutations.ReEncryptHierarchicalKeyInput(
+        item := newDecryptOnly,
+        originalKmsArn := localInput.mutationToApply.Terminal.kmsArn,
+        terminalKmsArn := localInput.mutationToApply.Terminal.kmsArn,
+        terminalEncryptionContext := ActiveEncryptionContext,
+        keyManagerStrategy := localInput.input.keyManagerStrategy
+      );
+      newActive :- Mutations.ReEncryptHierarchicalKey(
+        input := input,
+        localOperation := "InitializeMutation",
+        createNewActive := true);
+    }
+
+    return Success(
+        InitializeMutationActiveOutput(
+          writeActive := KeyStoreTypes.OverWriteEncryptedHierarchicalKey(Item:=newActive, Old:=localInput.activeItem),
+          writeVersion := KeyStoreTypes.WriteInitializeMutationVersion.rotate(rotate:=newDecryptOnly),
+          logStatements := [
+            Types.MutatedBranchKeyItem(ItemType := "Active: " + newVersion, Description := "Rotated"),
+            Types.MutatedBranchKeyItem(ItemType := "Decrypt Only: " + newVersion, Description := "Created")
+          ]
+        ));
+  }
+
+  method InitializeMutationActiveMutate(
+    localInput: InitializeMutationActiveInput
+  )
+    returns (output: Result<InitializeMutationActiveOutput, Types.Error>)
+    requires localInput.ValidState()
+    modifies localInput.Modifies
+    ensures localInput.ValidState()
+    requires localInput.input.DoNotVersion
+    ensures
+      output.Success?
+      ==>
+        && output.value.writeVersion.mutate?
+        && |output.value.logStatements| == 2
+  {
+    // Get the Active's Decrypt Only
+    var oldVersion := localInput.activeItem.Type.ActiveHierarchicalSymmetricVersion.Version;
+    var getOldReq := KeyStoreTypes.GetEncryptedBranchKeyVersionInput(
+      Identifier := localInput.input.Identifier,
+      Version := oldVersion);
+    var getOldRes? := localInput.input.storage.GetEncryptedBranchKeyVersion(getOldReq);
+    var getOldRes :- getOldRes?.MapFailure(e => Types.Error.AwsCryptographyKeyStore(e));
+
+      // If custom storage, validate read Decrypt Only
+    :- Need(
+      || localInput.input.storage is DefaultKeyStorageInterface.DynamoDBKeyStorageInterface
+      || (
+           && Mutations.ValidateItemFromStorage?(
+                localInput.input.storage, getOldRes.Item,
+                identifier := localInput.input.Identifier,
+                logicalName := localInput.input.logicalKeyStoreName)
+           && Structure.DecryptOnlyHierarchicalSymmetricKey?(getOldRes.Item)
+           && getOldRes.Item.Type.HierarchicalSymmetricVersion?
+         ),
+      Types.KeyStoreAdminException(
+        message := "Version (Decrypt Only) Item read from storage is malformed! Version: "
+        + Structure.BRANCH_KEY_TYPE_PREFIX + oldVersion)
+    );
+
+    // Assert Decrypt Only is in Original
+    var oldDecrypt := Mutations.MatchItemToState(getOldRes.Item, localInput.mutationToApply);
+    :- Need(
+      oldDecrypt.itemOriginal?,
+      Types.UnexpectedStateException(
+        message := "Version (Decrypt Only) Item read from storage is not in the expected original state!"
+        + " Version: " + Structure.BRANCH_KEY_TYPE_PREFIX + oldVersion)
+    );
+
+    // Mutate the Active
+    var newActive :- Mutations.MutateItem(
+      localInput.activeItem,
+      localInput.mutationToApply,
+      localInput.input.keyManagerStrategy,
+      "InitializeMutation", false);
+    // Mutate the decryptOnly
+    var newDecrypt :- Mutations.MutateItem(
+      oldDecrypt.item,
+      localInput.mutationToApply,
+      localInput.input.keyManagerStrategy,
+      "InitializeMutation", false);
+    var writeVersion := KeyStoreTypes.OverWriteEncryptedHierarchicalKey(Item:=newDecrypt, Old:=oldDecrypt.item);
+    return Success(
+        InitializeMutationActiveOutput(
+          writeActive := KeyStoreTypes.OverWriteEncryptedHierarchicalKey(Item:=newActive, Old:=localInput.activeItem),
+          writeVersion := KeyStoreTypes.WriteInitializeMutationVersion.mutate(mutate:=writeVersion),
+          logStatements := [
+            Types.MutatedBranchKeyItem(ItemType := "Active: " + oldVersion, Description := "Mutated"),
+            Types.MutatedBranchKeyItem(ItemType := "Decrypt Only: " + oldVersion, Description := "Mutated")
+          ]
+        ));
   }
 }
